core/Negation.thy
@@ -15,37 +15,11 @@ fun bdd_not :: \<open>'l bdd \<Rightarrow> 'l bdd\<close> where
 lemma bdd_not_correct_aux:
   assumes \<open>well_formed_nl ns\<close> \<open>t \<in> uid ` set ns\<close>
   shows \<open>\<not>bdd_eval_aux ns a t \<longleftrightarrow> bdd_eval_aux (map negate ns) a t\<close>
-  using assms
-proof (induction ns arbitrary: t)
-  case Nil
-  then show ?case
-    by simp
-next
-  case (Cons n ns)
-  then show ?case
-    by (cases n; auto split:ptr.splits)
-qed
+  using assms by (induction ns arbitrary: t rule: nl_induct) (auto split: ptr.splits)
 
 theorem bdd_not_correct:
   assumes \<open>well_formed bdd\<close>
   shows \<open>\<not>bdd_eval bdd a \<longleftrightarrow> bdd_eval (bdd_not bdd) a\<close>
-  apply (cases bdd rule:bdt_of_bdd.cases)
-  apply simp
-  using assms
-  apply simp
-  subgoal premises assms for ns
-    using assms
-    apply (cases ns)
-    apply (simp)
-    subgoal for root ns'
-      apply (cases root)
-      using bdd_not_correct_aux
-      apply (auto split:ptr.splits)
-      done
-    done
-  using assms
-  apply simp
-  done
-
+  using assms bdd_not_correct_aux by (cases bdd rule: bdd_cases) (auto split:ptr.splits)
 
 end
